src/Arrays.v
@@ -1,3 +1,4 @@
+Require Import List.
 Require Import Nomega NArith Word PropX PropXTac Memory SepIL IL.
 
 Require Import sep.Array Allocated.
@@ -60,8 +61,6 @@ Qed.
 
 Hint Resolve containsArray_goodSize.
 
-Require Import NArith Nomega.
-
 Lemma bound_N_nat : forall n,
   (n < pow2 32)%nat
   -> (N.of_nat n < Npow2 32)%N.
@@ -109,8 +108,6 @@ Section next.
 End next.
 
 Hint Resolve next.
-
-Require Import List.
 
 Lemma updN_app : forall b v a,
   Array.updN (a ++ b) (Datatypes.length a) v
@@ -305,7 +302,9 @@ Local Opaque mult.
 
 Lemma ptsto32m'_implies : forall specs stn p ws offset m,
   interp specs (ptsto32m' _ p offset ws stn m --->
-    [| arrayImplies (fun n => smem_get_word (implode stn) (p ^+ $(n)) m) ws offset |])%PropX.
+    [| arrayImplies (fun n => smem_read_word stn (p ^+ $(n)) m) ws offset |])%PropX.
+Proof.
+Admitted. (*
   induction ws; unfold ptsto32m', arrayImplies; fold ptsto32m'; fold arrayImplies; intuition.
   apply Imply_I; apply Inj_I; constructor.
   unfold starB, star; apply Imply_I.
@@ -326,64 +325,11 @@ Lemma ptsto32m'_implies : forall specs stn p ws offset m,
   eauto.
   eapply And_E2; eapply And_E2; apply Env; hnf; eauto.
 Qed.
-
-Theorem Himp_star_comm : forall P Q, (star P Q) ===> (star Q P).
-  intros; intro cs; apply himp_star_comm.
-Qed.
-
-Theorem Himp_ex_c : forall T (P : T -> _) Q, 
-  (exists v, Q ===> (P v)) -> Q ===> (ex P).
-  intros; intro cs; apply himp_ex_c; firstorder.
-Qed.
-
-Theorem Himp_ex_star : forall T (P : T -> _) Q,
-  (star (ex P) Q) ===> (ex (fun x => star (P x) Q)).
-  intros; intro cs; apply himp_ex_star.
-Qed.
-
-Theorem Himp'_ex : forall T (P : T -> _) Q,
-  (forall x, (P x) ===> Q) ->
-  ex P ===> Q.
-  intros; intro cs; apply himp'_ex; firstorder.
-Qed.
-
-Theorem Himp_star_frame : forall P Q R S, 
-  P ===> Q -> R ===> S -> (star P R) ===> (star Q S).
-  intros; intro cs; apply himp_star_frame; auto.
-Qed.
-
-
-Theorem Himp_star_pure_c : forall P Q (F : Prop),
-  (F -> P ===> Q) -> (star (inj (PropX.Inj F)) P) ===> Q.
-  intros; intro; apply himp_star_pure_c; firstorder.
-Qed.
-
-Theorem Himp_star_assoc : forall P Q R,
-  (star (star P Q) R) ===> (star P (star Q R)).
-  intros; intro; apply himp_star_assoc.
-Qed.
-
-Theorem Himp_star_assoc' : forall P Q R,
-  (star P (star Q R)) ===> (star (star P Q) R).
-  intros; intro cs.
-  destruct (heq_star_assoc cs P Q R); auto.
-Qed.
-
-Theorem Himp_star_Emp' : forall P,
-  P ===> Emp * P.
-  intros; intro cs.
-  destruct (heq_star_emp_l cs P); auto.
-Qed.
-
-Theorem Himp_star_pure_cc : forall P Q (p : Prop),
-  p ->
-  P ===> Q ->
-  P ===> (star (inj (PropX.Inj p)) Q).
-  intros; intro; eapply himp_star_pure_cc; eauto.
-Qed.
+*)
 
 Theorem ptsto32m'_in : forall a vs offset,
   ptsto32m _ a offset vs ===> ptsto32m' _ a offset vs.
+Proof.
   induction vs; intros.
 
   apply Himp_refl.
@@ -395,37 +341,37 @@ Theorem ptsto32m'_in : forall a vs offset,
            end) with (a ^+ $(offset)) by (destruct offset; W_eq).
   destruct vs.
   simpl ptsto32m'.
-  eapply Himp_trans; [ | apply Himp_star_comm ].
-  apply Himp_star_Emp'.
+  etransitivity. eapply STK.himp_star_emp_c.  apply STK.himp_star_comm.
 
-  apply Himp_star_frame; [ apply Himp_refl | ].
-  auto.
+  apply STK.himp_star_frame; [ reflexivity | ]. eapply IHvs.
 Qed.
 
 Lemma ptsto32m_implies : forall specs stn m p ws offset,
   interp specs (ptsto32m _ p offset ws stn m --->
-    [| arrayImplies (fun n => smem_get_word (implode stn) (p ^+ $(n)) m) ws offset |])%PropX.
+    [| arrayImplies (fun n => smem_read_word stn (p ^+ $(n)) m) ws offset |])%PropX.
   intros; eapply Imply_trans; apply ptsto32m'_implies || apply ptsto32m'_in.
 Qed.
 
 Lemma array_implies : forall specs stn m ws p,
   interp specs (array ws p stn m --->
-    [| arrayImplies (fun n => smem_get_word (implode stn) (p ^+ $(n)) m) ws 0 |])%PropX.
+    [| arrayImplies (fun n => smem_read_word stn (p ^+ $(n)) m) ws 0 |])%PropX.
   intros; apply ptsto32m_implies.
 Qed.
 
 Lemma arrayImplies_equal : forall stn p m m1 m2 m1' m2',
-  HT.split m m1 m2
-  -> HT.split m m1' m2'
+     split m m1 m2
+  -> split m m1' m2'
   -> forall ws ws' offset,
-    arrayImplies (fun n => smem_get_word (implode stn) (p ^+ $(n)) m1) ws offset
-    -> arrayImplies (fun n => smem_get_word (implode stn) (p ^+ $(n)) m1') ws' offset
+    arrayImplies (fun n => smem_read_word stn (p ^+ $(n)) m1) ws offset
+    -> arrayImplies (fun n => smem_read_word stn (p ^+ $(n)) m1') ws' offset
     -> length ws' = length ws
     -> ws' = ws.
+Proof.
   induction ws; destruct ws'; unfold length, arrayImplies; fold length; fold arrayImplies; intuition.
   f_equal; eauto.
-  eapply split_smem_get_word in H0; [ | eauto ].
-  eapply split_smem_get_word in H; [ | eauto ].
+  unfold smem_read_word in *.
+  eapply MSMF.split_multi_read in H0; [ | eauto ].
+  eapply MSMF.split_multi_read in H; [ | eauto ].
   congruence.
 Qed.
 
@@ -433,6 +379,8 @@ Lemma array_equals : forall specs stn st ws p fr ws' fr',
   interp specs (![array ws p * fr] (stn, st))
   -> interp specs (![array ws' p * fr'] (stn, st) --->
     [| length ws' = length ws -> ws' = ws |])%PropX.
+Proof.
+(*
   rewrite sepFormula_eq; unfold sepFormula_def, starB, star; simpl; intros.
   propxFo.
   eapply Imply_sound in H; [ | apply array_implies ].
@@ -449,7 +397,8 @@ Lemma array_equals : forall specs stn st ws p fr ws' fr',
   apply Inj_I; intro.
   eauto using arrayImplies_equal.
   eapply And_E1; eapply And_E2; apply Env; simpl; eauto.
-Qed.
+*)
+Admitted.
 
 Lemma imply_and : forall pc state (specs : codeSpec pc state) (P : Prop) Q R,
   (P -> interp specs (Q ---> R)%PropX)
@@ -463,7 +412,9 @@ Qed.
 Lemma smem_read_correctx'' : forall cs base stn ws offset i m,
   (i < length ws)%nat
   -> interp cs (ptsto32m' _ base (offset * 4) ws stn m
-    ---> [| smem_get_word (implode stn) (base ^+ $((offset + i) * 4)) m = Some (selN ws i) |])%PropX.
+    ---> [| smem_read_word stn (base ^+ $((offset + i) * 4)) m = Some (selN ws i) |])%PropX.
+Proof.
+(*
   induction ws.
 
   simpl length.
@@ -485,7 +436,7 @@ Lemma smem_read_correctx'' : forall cs base stn ws offset i m,
   eapply Inj_E; [ eapply And_E1; apply Env; hnf; eauto | intro ].
   eapply Inj_E; [ eapply And_E1; eapply And_E2; apply Env; hnf; eauto | intro ].
   apply Inj_I.
-  eapply split_smem_get_word; eauto.
+  eapply split_smem_read_word; eauto.
   tauto.
 
   unfold starB, star.
@@ -503,15 +454,18 @@ Lemma smem_read_correctx'' : forall cs base stn ws offset i m,
   apply interp_weaken; apply inj_imply.
   instantiate (1 := S offset).
   intros.
-  eapply split_smem_get_word; eauto.
+  eapply split_smem_read_word; eauto.
   hnf.
   do 2 eapply And_E2; apply Env; hnf; eauto.
-Qed.
+*)
+Admitted.
 
 Lemma array_boundx' : forall cs base stn ws m i,
   (0 < i < length ws)%nat
   -> base ^+ $(i * 4) = base
   -> interp cs (ptsto32m' _ base 0 ws stn m ---> [| False |])%PropX.
+Proof.
+(*
   destruct ws; simpl length; intros.
 
   elimtype False; omega.
@@ -543,11 +497,14 @@ Lemma array_boundx' : forall cs base stn ws m i,
   intro.
   apply Inj_I.
   destruct H4.
-  eapply smem_get_word_disjoint; eauto.
-Qed.
+  eapply smem_read_word_disjoint; eauto.
+*)
+Admitted.
 
 Lemma array_boundx : forall cs ws base stn m,
   interp cs (array ws base stn m ---> [| length ws < pow2 32 |]%nat)%PropX.
+Proof.
+(*
   intros.
   destruct (lt_dec (length ws) (pow2 32)); auto.
   apply Imply_I; apply Inj_I; auto.
@@ -568,11 +525,14 @@ Lemma array_boundx : forall cs ws base stn m,
   rewrite roundTrip_0.
   rewrite plus_0_r.
   apply natToWord_wordToNat.
-Qed.
+*)
+Admitted.
 
 Theorem containsArray_boundx' : forall cs P stn ls,
   containsArray P ls
   -> forall st, interp cs (P stn st ---> [|length ls < pow2 32|]%nat)%PropX.
+Proof.
+(*
   induction 1; intros.
   eapply array_boundx; eauto.
 
@@ -591,11 +551,13 @@ Theorem containsArray_boundx' : forall cs P stn ls,
   do 2 eapply And_E2; apply Env; simpl; eauto.
 
   rewrite upd_length in *; eauto.
-Qed.
+*)
+Admitted.
 
 Theorem containsArray_boundx : forall cs P stn ls st,
   containsArray P ls
   -> interp cs (![P] (stn, st) ---> [| length ls < pow2 32 |]%nat)%PropX.
+Proof.
   rewrite sepFormula_eq; intros; unfold sepFormula_def, fst, snd;
     auto using containsArray_boundx'.
 Qed.
