src/SepTheoryPropX.v
@@ -1,0 +1,196 @@
+Require Import RelationClasses.
+Require Import Heaps.
+Require Import PropX PropXTac.
+Require Import MirrorShard.SepTheory.
+Require Import MirrorShard.Heaps.
+Require IL.
+
+Set Implicit Arguments.
+Set Strict Implicit.
+
+Module Type PcSt.
+  Parameter pcType : Type.
+  Parameter stateType : Type.
+End PcSt.
+
+(** We make this transparent, so that clients can get at 
+ ** [ihprop] and it associated lemmas
+ **)
+Module SepTheoryPropX_Kernel (SM : SeparationMemory) (PC_ST : PcSt) <: 
+  SepTheory_Kernel 
+  with Definition hprop := 
+         IL.settings -> SM.smem -> PropX PC_ST.pcType PC_ST.stateType
+  with Definition himp := 
+         fun (gl gr : IL.settings -> SM.smem -> PropX PC_ST.pcType PC_ST.stateType) =>
+           forall cs stn m, interp cs (gl stn m ---> gr stn m).
+
+  Import PC_ST.
+
+  Definition ihprop (sos : list Type) : Type :=
+    IL.settings -> SM.smem -> propX PC_ST.pcType PC_ST.stateType sos.
+
+  Definition hprop : Type := ihprop nil.
+
+  Definition himp : ihprop nil -> ihprop nil -> Prop := 
+    fun gl gr =>
+      forall cs stn m, interp cs (gl stn m ---> gr stn m).
+
+  Global Instance Refl_himp : Reflexive himp.
+  Proof.
+    red; unfold himp; intros. 
+    eapply Imply_I; eauto.
+  Qed.
+  Global Instance Trans_himp : Transitive himp.
+  Proof.
+    red; unfold himp; firstorder.
+    eapply Imply_I. eapply Imply_E. eapply valid_weaken. eapply H0. firstorder.
+    eapply Imply_E. eapply valid_weaken. eapply H. firstorder. eauto.
+  Qed.
+
+  Section with_sos.
+    Variable sos : list Type.
+
+    (* Definitions *)
+    Definition iinjX (p : propX pcType stateType sos) : ihprop sos :=
+      fun _ m => PropX.And p (PropX.Inj (m = SM.smem_emp)).
+
+    Definition iinj (p : Prop) : ihprop sos := iinjX (PropX.Inj p).
+
+    Definition iemp : ihprop sos := iinj True.
+
+    Definition istar (l r : ihprop sos) : ihprop sos :=
+      fun s m => PropX.Exists (fun ml : SM.smem => PropX.Exists (fun mr : SM.smem =>
+        PropX.And (PropX.Inj (SM.split m ml mr)) (And (l s ml) (r s mr)))).
+
+    Definition iex (T : Type) (p : T -> ihprop sos) : ihprop sos :=
+      fun s h => PropX.Exists (fun t => p t s h).
+
+    Definition ihptsto (p : SM.M.addr) (v : SM.M.value) : ihprop sos :=
+      fun s h =>
+        PropX.Inj (SM.smem_get p h = Some v /\ forall p', p' <> p -> SM.smem_get p' h = None).
+  End with_sos.
+    
+
+  (* Definitions *)
+  Definition injX := @iinjX nil.
+
+  Definition inj := @iinj nil.
+
+  Definition emp := @iemp nil.
+
+  Definition star := @istar nil.
+
+  Definition ex := @iex nil.
+
+  Definition hptsto := @ihptsto nil. 
+
+  Ltac unfold_all := 
+    unfold ex, star, emp, inj, injX, iex, istar, iemp, iinj, iinjX, himp, interp.
+
+  Require Import PropXRel.
+  
+  Hint Immediate SM.split_comm : heaps.
+  Hint Resolve SM.split_assoc : heaps.
+  
+  Lemma himp_star_comm : forall P Q, himp (star P Q) (star Q P).
+  Proof.
+    unfold_all; intros; propxIntuition.
+    do 2 eapply Exists_I. propxIntuition; eauto using SM.split_comm.
+  Qed.
+
+  Theorem himp_star_assoc : forall P Q R,
+    himp (star (star P Q) R) (star P (star Q R)).
+  Proof.      
+    unfold_all; intros; propxIntuition.
+    destruct (SM.split_assoc _ _ _ _ _ H H0). clear H H0. destruct H1.
+    do 2 eapply Exists_I; propxIntuition. eauto. do 2 eapply Exists_I. propxIntuition. eauto.
+  Qed.
+
+  Theorem himp_star_emp_p : forall P : hprop, himp (star emp P) P.
+  Proof.
+    unfold_all; intros; propxIntuition.
+    subst. eapply SM.split_emp in H. subst; propxIntuition.
+  Qed.
+
+  Theorem himp_star_emp_c : forall P : hprop, himp P (star emp P).
+  Proof.
+    unfold_all; intros; propxIntuition.
+    do 2 eapply Exists_I. instantiate (1 := m). instantiate (1 := SM.smem_emp).
+    propxIntuition; auto. eapply SM.split_emp; auto.
+  Qed.
+
+  Theorem himp_star_frame : forall P Q R S, 
+    himp P Q -> himp R S -> himp (star P R) (star Q S).
+  Proof.
+    unfold_all; intros; propxIntuition.
+    do 2 eapply Exists_I. propxIntuition. eassumption.
+    eapply Imply_E. eapply valid_weaken. eapply H. firstorder. propxIntuition.
+    eapply Imply_E. eapply valid_weaken. eapply H0. firstorder. propxIntuition.
+  Qed.
+
+  Theorem himp_star_pure_p :
+    forall (P Q : hprop) (F : Prop),
+      himp (star (inj F) P) Q -> F -> himp P Q.
+  Proof.
+    unfold_all; intros; propxIntuition.
+    specialize (H cs stn m). 
+    eapply Imply_E. eapply valid_weaken. eapply H. firstorder.
+    do 2 eapply Exists_I; propxIntuition. eapply SM.split_emp; auto. auto. reflexivity.
+  Qed.
+
+  Theorem himp_star_pure_c :
+    forall (P Q : hprop) (F : Prop),
+      (F -> himp P Q) -> himp (star (inj F) P) Q.
+  Proof.
+    unfold_all; intros; propxIntuition.
+    propxIntuition. eapply Imply_E.
+    eapply valid_weaken. eapply H; auto. firstorder.
+    subst. eapply SM.split_emp in H0. subst.
+    constructor; firstorder.
+  Qed.
+
+  Theorem himp_star_pure_cc :
+    forall (P Q : hprop) (p : Prop),
+      p -> himp P Q -> himp P (star (inj p) Q).
+  Proof.
+    unfold_all; intros; propxIntuition.
+    do 2 eapply Exists_I; propxIntuition.
+    2: eauto. 2: reflexivity. eapply SM.split_emp; reflexivity.
+    eapply Imply_E. eapply valid_weaken. eapply H0. firstorder.
+    constructor; firstorder.
+  Qed.
+
+  Theorem himp_ex_p :
+    forall (T : Type) (P : T -> hprop) (Q : hprop),
+      (forall v : T, himp (P v) Q) -> himp (ex P) Q.
+  Proof.
+    unfold_all; intros; propxIntuition.
+    eapply Imply_E. eapply valid_weaken. eapply H. firstorder. constructor; firstorder.
+  Qed.
+  
+  Theorem himp_ex_c :
+    forall (T : Type) (P : T -> hprop) (Q : hprop),
+      (exists v : T, himp Q (P v)) -> himp Q (ex P).
+  Proof.
+    unfold_all; intros; propxIntuition.
+    destruct H. eapply Exists_I.
+    instantiate (1 := x). eapply Imply_E.
+    eapply valid_weaken; try eapply H. firstorder. constructor; firstorder.
+  Qed.
+
+  Theorem himp_ex_star : forall T (P : T -> _) Q,
+    himp (star (ex P) Q) (ex (fun x => star (P x) Q)).
+  Proof.
+    unfold_all; intros; propxIntuition.
+    eapply Exists_I with (B := x1). do 2 eapply Exists_I. propxIntuition; auto.
+  Qed.
+
+  Theorem himp_star_ex : forall T (P : T -> _) Q,
+    himp (ex (fun x => star (P x) Q)) (star (ex P) Q).
+  Proof.
+    unfold_all; intros; propxIntuition.
+    do 2 eapply Exists_I; propxIntuition; eauto.
+    eapply Exists_I; propxIntuition.
+  Qed.
+  
+End SepTheoryPropX_Kernel.
